scratch/print_methods.go
@@ -1,0 +1,16 @@
+package main
+
+import (
+	"fmt"
+	"reflect"
+	"github.com/dafny-lang/DafnyRuntimeGo/v4/dafny"
+)
+
+func main() {
+	var seq dafny.Sequence
+	t := reflect.TypeOf(&seq).Elem()
+	for i := 0; i < t.NumMethod(); i++ {
+		m := t.Method(i)
+		fmt.Printf("Method %s: %s\n", m.Name, m.Type)
+	}
+}
