scratch/go.mod
@@ -1,0 +1,5 @@
+module scratch
+
+go 1.26.4
+
+require github.com/dafny-lang/DafnyRuntimeGo/v4 v4.11.3 // indirect
